isabelle/Chapter16_3_Typechecking.thy
@@ -4,10 +4,6 @@ begin
 
 inductive typecheck :: "type env => expr => type => bool"
 where tc_var [simp]: "lookup gam x = Some t ==> typecheck gam (Var x) t"
-    | tc_zero [simp]: "typecheck gam Zero Nat"
-    | tc_suc [simp]: "typecheck gam e Nat ==> typecheck gam (Suc e) Nat"
-    | tc_isz [simp]: "typecheck gam et Nat ==> typecheck gam e0 t ==> 
-                typecheck (extend gam Nat) es t ==> typecheck gam (IsZ et e0 es) t"
     | tc_lam [simp]: "typecheck (extend gam t1) e t2 ==> typecheck gam (Lam t1 e) (Arrow t1 t2)"
     | tc_appl [simp]: "typecheck gam e1 (Arrow t2 t) ==> typecheck gam e2 t2 ==> 
                 typecheck gam (Appl e1 e2) t"
@@ -27,9 +23,6 @@ where tc_var [simp]: "lookup gam x = Some t ==> typecheck gam (Var x) t"
                 typecheck gam (Unfold e) (type_subst (Rec t) t)"
 
 inductive_cases [elim!]: "typecheck gam (Var x) t"
-inductive_cases [elim!]: "typecheck gam Zero t"
-inductive_cases [elim!]: "typecheck gam (Suc e) t"
-inductive_cases [elim!]: "typecheck gam (IsZ et e0 es) t"
 inductive_cases [elim!]: "typecheck gam (Lam t1 e) t"
 inductive_cases [elim!]: "typecheck gam (Appl e1 e2) t"
 inductive_cases [elim!]: "typecheck gam Triv t"
